finish part1

heap/list_relation.v
@@ -3,8 +3,8 @@ Require Import FloydSeq.proofauto.
 Require Import Notations Logic Datatypes.
 Require Export Coq.Classes.Init.
 (* Require Import Coq.Program.Basics. *)
-Require Import Coq.Program.Tactics.
-Require Import Coq.Relations.Relation_Definitions.
+(* Require Import Coq.Program.Tactics.
+Require Import Coq.Relations.Relation_Definitions. *)
 From Coq Require Import String List ZArith. 
 From compcert Require Import Coqlib Integers Floats AST Ctypes Cop Clight Clightdefs.
 
@@ -17,9 +17,10 @@ Local Open Scope list_scope.
 Require Import SetsClass.SetsClass.
 Local Open Scope sets.
 Import SetsNotation.
-Lemma list_equal : forall (A: Type) (l1 l2: list A) (d: A),
-  l1 = l2 <-> length l1 = length l2 /\
-  forall (i: nat), (i < length l1)%nat -> nth i l1 d = nth i l2 d.
+
+Lemma list_equal : forall (A: Type) (l1 l2: list A) {d: Inhabitant A},
+  l1 = l2 <-> Zlength l1 = Zlength l2 /\
+  forall (i: Z), 0 <= i < Zlength l1 -> Znth i l1 = Znth i l2.
 Proof.
   split.
   + intros.
@@ -27,66 +28,67 @@ Proof.
     tauto.
   + intros.
     destruct H.
-    apply (nth_ext l1 l2 d d); [tauto | tauto].
+    apply (Znth_eq_ext l1 l2); [tauto | tauto].
 Qed.
 
-Definition list_swap (x: nat) (y: nat):
+Definition list_swap (x: Z) (y: Z):
   list Z -> list Z -> Prop :=
   fun l1 l2 =>
-    length l1 = length l2 /\
-    nth x l1 0 = nth y l2 0 /\ nth y l1 0 = nth x l2 0 /\
-    forall i, (i < length l1)%nat /\ i <> x /\ i <> y ->
-      nth i l1 0 = nth i l2 0.
+    Zlength l1 = Zlength l2 /\
+    Znth x l1 = Znth y l2 /\ Znth y l1 = Znth x l2 /\
+    forall i, 0 <= i < Zlength l1 /\ i <> x /\ i <> y ->
+      Znth i l1 = Znth i l2.
 
 Import ListNotations.
 
 Require Import BinNums.
 Require Coq.micromega.Lia.
 
-Definition list_state: Type := ((list Z) * nat).
+Definition list_state: Type := ((list Z) * Z).
 
 Definition get_list_val(l: list_state): Z := 
-  nth ((snd l)) (fst l) 0.
+  Znth ((snd l)) (fst l).
 
 Definition legal_list_state(l: list_state): Prop:=
-  ((snd l) <= (length (fst l)))%nat /\ (1%nat <= (snd l))%nat.
+  ((snd l) < Zlength (fst l)) /\ 1 <= (snd l).
 
 Definition list_up_succeed:
   list_state -> list_state -> Prop :=
   fun l1 l2 => legal_list_state l1 /\ legal_list_state l2 /\
-    (1%nat < (snd l1))%nat /\ ((snd l2) = (snd l1)/2)%nat /\
-    get_list_val l1 > (nth (snd l2) (fst l1) 0) /\
+    1 < (snd l1) /\ (snd l2) = (snd l1) / 2 /\
+    get_list_val l1 > (Znth (snd l2) (fst l1)) /\
     (list_swap (snd l1) (snd l2) (fst l1) (fst l2)).
 
 Definition list_up_fail:
   list_state -> list_state -> Prop:=
   Rels.test(fun l =>  legal_list_state l /\
-    ((1%nat = (snd l))%nat \/
-    ((1%nat < (snd l))%nat /\ 
-    get_list_val l <= (nth ((snd l)/2) (fst l) 0)))).
+    (1 = (snd l) \/
+    (1 < (snd l) /\ 
+    get_list_val l <= (Znth ((snd l) / 2) (fst l))))).
 
-Fixpoint iter_n_list_up (n: nat):
+(* Fixpoint iter_n_list_up (n: nat):
   list_state -> list_state -> Prop :=
   match n with
   | O => list_up_fail
   | S n0 => list_up_succeed ∘ (iter_n_list_up n0)
-  end.
+  end. *)
 
 Definition heap_list_up:
   list_state -> list_state -> Prop :=
-  ⋃ (iter_n_list_up).
+  (clos_refl_trans list_up_succeed) ∘ list_up_fail.
+  (* ⋃ (iter_n_list_up). *)
 
 Definition left_son(l: list_state): list_state :=
-  pair (fst l) ((snd l) * 2)%nat.
+  pair (fst l) (2 * (snd l)).
 
 Definition left_son_swap(l1 l2: list_state): Prop :=
-  (list_swap (snd l1) (snd l2) (fst l1) (fst l2)) /\ ((snd l1) * 2 = (snd l2))%nat.
+  (list_swap (snd l1) (snd l2) (fst l1) (fst l2)) /\ 2 * (snd l1) = (snd l2).
   
 Definition right_son_swap(l1 l2: list_state): Prop :=
-  (list_swap (snd l1) (snd l2) (fst l1) (fst l2)) /\ ((snd l1) * 2 + 1 = (snd l2))%nat.
+  (list_swap (snd l1) (snd l2) (fst l1) (fst l2)) /\ 2 * (snd l1) + 1 = (snd l2).
 
 Definition right_son(l: list_state): list_state :=
-  pair (fst l) ((snd l) * 2 + 1)%nat.
+  pair (fst l) (2 * (snd l) + 1).
 
 Definition left_son_check_list (l: list_state): Prop :=
   legal_list_state (left_son l) /\
@@ -101,8 +103,8 @@ Definition list_down_succeed:
   fun l1 l2 =>
     ((left_son_check_list l1) /\ ~(right_son_check_list l1) /\ (left_son_swap l1 l2)) \/
     ((left_son_check_list l1) /\ (right_son_check_list l1) /\ (
-      ((get_list_val (left_son l1)) > (get_list_val (right_son l1)) /\ (left_son_swap l1 l2))  \/
-      ((get_list_val (left_son l1)) <= (get_list_val (right_son l1)) /\ (right_son_swap l1 l2))
+      ((get_list_val (left_son l1)) >= (get_list_val (right_son l1)) /\ (left_son_swap l1 l2))  \/
+      ((get_list_val (left_son l1)) < (get_list_val (right_son l1)) /\ (right_son_swap l1 l2))
     )) \/
     (~(left_son_check_list l1) /\ (right_son_check_list l1) /\ (right_son_swap l1 l2)).
 
@@ -111,32 +113,41 @@ Definition list_down_fail:
   Rels.test(fun l =>
     ~(left_son_check_list l) /\ ~(right_son_check_list l)).
 
-Fixpoint iter_n_list_down (n: nat):
+(* Fixpoint iter_n_list_down (n: nat):
   list_state -> list_state -> Prop :=
   match n with
   | O => list_down_fail
   | S n0 => list_down_succeed ∘ (iter_n_list_down n0)
-  end.
+  end. *)
 
 Definition heap_list_down:
   list_state -> list_state -> Prop :=
-  ⋃ (iter_n_list_down).
+  (clos_refl_trans list_down_succeed) ∘ list_down_fail.
+  (* ⋃ (iter_n_list_down). *)
+
+Ltac simpl_Z :=
+  simpl; unfold Zlength, Zlength_aux; unfold Znth; simpl.
 
 Ltac try_list_unfold :=
   unfold left_son_check_list; unfold left_son_swap; unfold left_son; 
   unfold right_son_check_list; unfold right_son_swap; unfold right_son;
+  unfold get_list_val; unfold legal_list_state; simpl_Z.
+
+Ltac try_list_unfold_witout_Z :=
+  unfold left_son_check_list; unfold left_son_swap; unfold left_son; 
+  unfold right_son_check_list; unfold right_son_swap; unfold right_son;
   unfold get_list_val; unfold legal_list_state; simpl.
 
-Example test : list_swap 2%nat 1%nat [2; 3; 4; 5] [2; 4; 3; 5].
+Example test : list_swap 2 1 [2; 3; 4; 5] [2; 4; 3; 5].
 Proof.
   unfold list_swap.
-  unfold length.
-  unfold nth at 1 2 3 4.
+  unfold Zlength, Zlength_aux.
+  unfold Znth at 1 2 3 4.
   split; [tauto | ].
   split; [tauto | ].
   split; [tauto | ].
   intros.
-  assert (i = 0%nat \/ i = 3%nat) by lia.
+  assert (i = 0 \/ i = 3) by lia.
   destruct H0.
   + rewrite H0.
     tauto.
@@ -144,92 +155,100 @@ Proof.
     tauto.  
 Qed.
 
-Example check_succeed_up : list_up_succeed (pair [233;2; 3; 4; 5] 2%nat) (pair [233;3; 2; 4; 5] 1%nat).
+Example check_succeed_up : list_up_succeed (pair [233;2; 3; 4; 5] 2) (pair [233;3; 2; 4; 5] 1).
 Proof.
   unfold list_up_succeed.
-  split; [unfold legal_list_state; simpl; lia|].
-  split; [unfold legal_list_state; simpl; lia|].
+  split; [unfold legal_list_state; simpl_Z; lia|].
+  split; [unfold legal_list_state; simpl_Z; lia|].
   split; [simpl; lia|].
   split; [simpl; tauto|].
-  split; [unfold get_list_val; simpl; lia|].
+  split; [unfold get_list_val; simpl_Z; lia|].
   simpl.
-  unfold list_swap. unfold length.
+  unfold list_swap. simpl_Z.
   split; [tauto|].
   split; [tauto|].
   split; [tauto|].
   intros.
   destruct H as [H0 [H1 H2]].
-  assert (i = 0%nat \/ i = 3%nat \/ i = 4%nat) by lia.
+  assert (i = 0 \/ i = 3 \/ i = 4) by lia.
   destruct H;[ subst; tauto|].
   destruct H; subst; tauto.
 Qed.
 
-Example check_heap_list_up : heap_list_up (pair [233;2; 3; 4; 5] 2%nat) (pair [233;3; 2; 4; 5] 1%nat).
+Example check_heap_list_up : heap_list_up (pair [233;2; 3; 4; 5] 2) (pair [233;3; 2; 4; 5] 1).
 Proof.
   unfold heap_list_up.
   unfold_RELS_tac.
-  exists 1%nat.
-  unfold iter_n_list_up.
-  unfold_RELS_tac.
-  exists (pair [233;3; 2; 4; 5] 1%nat).
+  exists (pair [233;3; 2; 4; 5] 1).
   split.
-  + apply check_succeed_up.
+  + exists 1%nat.
+    unfold list_up_succeed.
+    unfold nsteps.
+    unfold_RELS_tac.
+    exists (pair [233;3; 2; 4; 5] 1).
+    try_list_unfold.
+    split; [|reflexivity].
+    split; [lia|]. split; [lia|]. split; [lia|].
+    split; [reflexivity|].
+    split; [lia|].
+    unfold list_swap.
+    split; [tauto|]. split; [tauto|]. split; [tauto|].
+    unfold Zlength, Zlength_aux; simpl.
+    intros.
+    destruct H, H, H0.
+    assert (i = 0 \/ i = 3 \/ i = 4) by lia.
+    destruct H3; [subst; reflexivity|].
+    destruct H3; subst; reflexivity.
   + unfold list_up_fail.
-    simpl.
-    split.
-    - split; unfold legal_list_state; simpl; lia.
-    - tauto.
+    unfold_RELS_tac.
+    try_list_unfold.
+    split; [|reflexivity].
+    split; [lia|].
+    left; reflexivity.
 Qed.
 
-Example check_heap_list_up2 : heap_list_up (pair [233;100;3;2;5] 4%nat) (pair [233;100;5;2;3] 2%nat).
+Example check_heap_list_up2 : heap_list_up (pair [233;100;3;2;5] 4) (pair [233;100;5;2;3] 2).
 Proof.
   unfold heap_list_up.
   unfold_RELS_tac.
-  exists 1%nat.
-  unfold iter_n_list_up.
-  unfold_RELS_tac.
-  exists (pair [233;100;5;2;3] 2%nat).
+  exists (pair [233;100;5;2;3] 2).
   split.
-  + unfold list_up_succeed.
-    split; [unfold legal_list_state; simpl; lia|].
-    split; [unfold legal_list_state; simpl; lia|].
-    split; [unfold snd; lia|].
-    split; [unfold snd; tauto|].
-    split; [unfold get_list_val; simpl; lia|].
-    simpl.
-    unfold list_swap. unfold length.
-    split; [tauto|].
-    split; [tauto|].
-    split; [tauto|].
+  + exists 1%nat.
+    unfold nsteps.
+    unfold_RELS_tac.
+    exists (pair [233;100;5;2;3] 2).
+    split; [|reflexivity].
+    unfold list_up_succeed.
+    try_list_unfold.
+    split; [lia|]. split; [lia|]. split; [lia|].
+    split; [reflexivity|]. split; [lia|].
+    unfold list_swap. simpl_Z.
+    split; [tauto|]. split; [tauto|]. split; [tauto|].
     intros.
     destruct H as [H0 [H1 H2]].
-    assert (i = 0%nat \/ i = 1%nat \/ i = 3%nat) by lia.
+    assert (i = 0 \/ i = 1 \/ i = 3) by lia.
     destruct H;[ subst; tauto|].
     destruct H; subst; tauto.
   + unfold list_up_fail.
-    simpl.
-    split.
-    - split.
-      unfold legal_list_state; simpl; lia.
-      right; split; [lia|].
-      unfold get_list_val; simpl; lia.
-    - tauto.
+    unfold_RELS_tac.
+    try_list_unfold.
+    split; [split; lia |reflexivity].
 Qed.
 
-Example check_succeed_down : list_down_succeed (pair [233;4;6;9;2;4;1;3] 1%nat) (pair [233;9;6;4;2;4;1;3] 3%nat).
+Example check_succeed_down : list_down_succeed (pair [233;4;6;9;2;4;1;3] 1) (pair [233;9;6;4;2;4;1;3] 3).
 Proof.
   unfold list_down_succeed.
   right; left.
   split; try_list_unfold; [lia|].
   split; [lia|].
   right; split; [lia|].
-  unfold list_swap; unfold length.
+  unfold list_swap; simpl_Z.
   split; [|tauto].
   split; [tauto|].
   split; [tauto|].
   split; [tauto|].
   intros.
-  assert (i = 0%nat \/ i = 2%nat \/ i = 4%nat \/ i = 5%nat \/ i = 6%nat \/ i = 7%nat) by lia.
+  assert (i = 0 \/ i = 2 \/ i = 4 \/ i = 5 \/ i = 6 \/ i = 7) by lia.
   destruct H0; [subst; tauto|].
   destruct H0; [subst; tauto|].
   destruct H0; [subst; tauto|].
@@ -237,18 +256,20 @@ Proof.
   destruct H0; subst; tauto.
 Qed.
 
-
-Example check_heap_list_down : heap_list_down (pair [233;4;6;9;2;4;1;3] 1%nat) (pair [233;9;6;4;2;4;1;3] 3%nat).
+Example check_heap_list_down : heap_list_down (pair [233;4;6;9;2;4;1;3] 1) (pair [233;9;6;4;2;4;1;3] 3).
 Proof.
   unfold heap_list_down.
   unfold_RELS_tac.
-  exists 1%nat.
-  unfold iter_n_list_down.
-  unfold_RELS_tac.
-  exists ([233; 9; 6; 4; 2; 4; 1; 3], 3%nat).
+  exists (pair [233;9;6;4;2;4;1;3] 3).
   split.
-  + exact check_succeed_down.
+  + exists 1%nat.
+    unfold nsteps.
+    unfold_RELS_tac.
+    exists ([233; 9; 6; 4; 2; 4; 1; 3], 3).
+    split; [exact check_succeed_down|reflexivity].
   + unfold list_down_fail.
-    simpl; split; [|tauto].
-    try_list_unfold; lia.
+    unfold_RELS_tac.
+    split; [|reflexivity].
+    try_list_unfold.
+    lia.
 Qed.
