heap/definitions.v
@@ -1,0 +1,697 @@
+Require Import FloydSeq.proofauto.
+Require Import cprogs.heap.program.
+Require Import cprogs.heap.list_relation.
+
+Require Import Coq.micromega.Psatz.
+Require Import Coq.micromega.Lia.
+Require Import SetsClass.SetsClass.
+Require Import Classical_Prop.
+
+Instance CompSpecs : compspecs. make_compspecs prog. Defined.
+Definition Vprog : varspecs. mk_varspecs prog. Defined.
+
+Notation "'IntRepr'" := (Int.repr).
+Notation "'store_int' p x" :=
+  (@data_at CompSpecs Tsh tint (Vint(IntRepr(x))) p)
+  (x at level 0, p at level 0, at level 0).
+Notation "'store_int_array' p l size" :=
+  (@data_at CompSpecs Tsh (tarray tint size) (map Vint (map Int.repr l)) p)
+  (p at level 0, l at level 0, size at level 0, at level 0).
+
+(* Parameter MaxHeap : list Z -> Z -> Prop. *)
+(* Parameter MaxHeap_p : list Z -> Z -> Z -> Prop. *)
+(* Parameter shr : Z -> Z -> Z. *)
+
+(* Parameter up : list Z -> Z -> Z -> Z -> list Z. *)
+(* Parameter down : list Z -> Z -> Z -> Z -> list Z. *)
+(* Parameter push : list Z -> Z -> Z -> list Z. *)
+(* Parameter pop : list Z -> Z -> list Z. *)
+(* Parameter pop_length : list Z -> Z -> Z. *)
+(* Parameter pop_result : list Z -> Z -> Z. *)
+
+Import ListNotations.
+
+Lemma int_array_is_ptr: forall (p: val) (l: list Z) (size: Z),
+  !!(size >= 0) && store_int_array p l size |-- !!isptr p.
+Proof.
+  intros.
+  entailer!.
+Qed.
+
+Definition heap_push: list Z -> Z -> list Z -> Prop :=
+  fun l val l' =>
+    exists (p: Z), heap_list_up (pair (l ++ [val]) (Zlength l)) (pair l' p).
+
+Definition heap_pop: list Z -> list Z -> Prop :=
+  fun l l' => (Zlength l = 2 /\ Zlength l' = 1) \/ (
+    Zlength l > 2 /\
+    (exists (p: Z), heap_list_down (pair (firstn (Z.to_nat ((Zlength l) - 1)) (upd_Znth 1 l (Znth ((Zlength l) - 1) l))) 1) (pair l' p))).
+
+Lemma list_length: forall (p: val) (l: list Z) (size: Z),
+  !!(size >= 0) && store_int_array p l size |-- !!(Zlength l = size).
+Proof.
+  intros.
+  entailer!.
+  rewrite Zlength_map, Zlength_map.
+  reflexivity.
+Qed.
+
+Definition up: list Z -> Z -> Z -> Z -> list Z -> Prop :=
+  fun l size p0 p1 l' =>
+    heap_list_up ((firstn (Z.to_nat (size + 1)) l), p0) ((firstn (Z.to_nat (size + 1)) l'), p1).
+
+Definition up_inv: list Z -> Z -> Z -> Z -> list Z -> Prop :=
+  fun l size p0 p1 l' =>
+    (clos_refl_trans list_up_succeed) ((firstn (Z.to_nat (size + 1)) l), p0) ((firstn (Z.to_nat (size + 1)) l'), p1).
+
+Definition down: list Z -> Z -> Z -> Z -> list Z -> Prop :=
+  fun l size p0 p1 l' =>
+    heap_list_down ((firstn (Z.to_nat (size + 1)) l), p0) ((firstn (Z.to_nat (size + 1)) l'), p1).
+
+Definition down_inv: list Z -> Z -> Z -> Z -> list Z -> Prop :=
+  fun l size p0 p1 l' =>
+    (clos_refl_trans list_down_succeed) ((firstn (Z.to_nat (size + 1)) l), p0) ((firstn (Z.to_nat (size + 1)) l'), p1).
+
+Definition push: list Z -> Z -> Z -> list Z -> Prop :=
+  fun l size val l' =>
+    heap_push (firstn (Z.to_nat (size + 1)) l) val (firstn (Z.to_nat (size + 2)) l').
+
+Definition pop: list Z -> Z -> list Z -> Prop :=
+  fun l size l' =>
+    size = 0 /\ l = l' \/ size > 0 /\ heap_pop (firstn (Z.to_nat (size + 1)) l) (firstn (Z.to_nat size) l').
+
+Definition pop_length (l: list Z) (size: Z): Z :=
+  match size with
+    | 0 => 0
+    | _ => size - 1
+  end.
+
+Definition pop_result (l: list Z) (size: Z): Z :=
+  match size with
+    | 0 => -1
+    | _ => 0
+  end.
+
+Fixpoint all_int (l: list Z): Prop :=
+  match l with
+  | nil => True
+  | h :: l0 => Int.min_signed <= h <= Int.max_signed /\ all_int l0
+  end.
+
+Lemma all_int_app: forall (l1 l2: list Z),
+  all_int l1 -> all_int l2 -> all_int (l1 ++ l2).
+Proof.
+  intros.
+  induction l1; [tauto|].
+  rewrite <- app_comm_cons.
+  revert H.
+  unfold all_int; fold all_int.
+  intros.
+  destruct H.
+  split; tauto.
+Qed.
+
+Lemma all_int_sublist: forall (Hl: list Z) (l r: Z),
+  all_int Hl -> all_int (sublist l r Hl).
+Proof.
+  intros.
+  unfold sublist.
+  assert (forall (lt: list Z) (p: nat), all_int lt -> all_int (skipn p lt)). {
+    intros; revert lt H0.
+    induction p.
+    + unfold skipn; tauto.
+    + intros.
+      destruct lt; [rewrite skipn_nil; tauto|].
+      assert (skipn p lt = skipn (S p) (z :: lt)) by reflexivity.
+      rewrite <- H1.
+      unfold all_int in H0; fold all_int in H0.
+      destruct H0.
+      apply IHp; tauto.
+  }
+  assert (forall (lt: list Z) (p: nat), all_int lt -> all_int (firstn p lt)). {
+    intros; revert lt H1.
+    induction p.
+    + unfold firstn, all_int. tauto.
+    + intros.
+      destruct lt; [rewrite firstn_nil; tauto|].
+      assert (z :: firstn p lt = firstn (S p) (z :: lt)) by reflexivity.
+      rewrite <- H2.
+      revert H1.
+      unfold all_int; fold all_int; intros.
+      destruct H1.
+      split; [tauto|].
+      apply IHp; tauto.
+  }
+  apply H1.
+  apply H0.
+  tauto.
+Qed.
+
+Lemma all_int_Znth: forall (l: list Z) (p: Z),
+  all_int l -> 0 <= p < (Zlength l) -> 
+  Int.min_signed <= (Znth p l) <= Int.max_signed.
+Proof.
+  intros.
+  destruct H0.
+  assert (p + 1 <= Zlength l) by lia.
+  pose proof sublist_one p (p+1) l H0 H2 ltac:(lia).
+  pose proof all_int_sublist l p (p+1) H.
+  rewrite H3 in H4.
+  unfold all_int in H4.
+  tauto.
+Qed.
+
+Lemma all_int_upd_Znth: forall (l: list Z) (p val: Z),
+  all_int l ->
+  Int.min_signed <= val -> val <= Int.max_signed ->
+  all_int (upd_Znth p l val).
+Proof.
+  intros.
+  unfold upd_Znth.
+  apply all_int_app.
+  + apply all_int_sublist; tauto.
+  + unfold all_int; fold all_int.
+    split; [tauto|].
+    apply all_int_sublist; tauto.
+Qed.
+
+Lemma firstn_app_upd_Znth: forall (l: list Z) (val: Z) (pos: nat), 
+  (Z.of_nat pos) < Zlength l ->
+  firstn (pos + 1) (upd_Znth (Z.of_nat pos) l val) = (firstn pos l) ++ [val].
+Proof.
+  intros.
+  revert l H.
+  induction pos; intros; [tauto|].
+  destruct l; [discriminate|].
+  replace (upd_Znth (Z.of_nat (S pos)) (z :: l) val) with (z :: (upd_Znth (Z.of_nat pos) l val)).
+  + assert ( ((S pos) + 1 = S (pos +1))%nat ) by lia.
+    rewrite H0.
+    rewrite ! firstn_cons.
+    rewrite <- app_comm_cons.
+    rewrite Zlength_cons in H.
+    assert (Z.of_nat pos < Zlength l ) by lia.
+    pose proof (IHpos l H1).
+    rewrite H2.
+    reflexivity.
+  + assert (z::l = [z]++l) by reflexivity.
+    rewrite H0 in H.
+    assert (1<= (Z.of_nat (S pos)) <= Zlength ([z] ++ l)) by lia.
+    rewrite H0.
+    rewrite Zlength_app in H1.
+    pose proof (upd_Znth_app2 [z] l (Z.of_nat (S pos)) val H1).
+    rewrite H2.
+    replace (Z.of_nat pos) with (Z.of_nat (S pos) - Zlength [z]); [reflexivity|].
+    unfold Zlength; unfold Zlength_aux.
+    lia.
+Qed.
+
+Lemma left_son_check_hold: forall l pos len1 len2,
+  len2 <= len1 -> len2 >= 1 ->
+  ~left_son_check_list (firstn (Z.to_nat len1) l, pos) ->
+  ~left_son_check_list (firstn (Z.to_nat len2) l, pos).
+Proof.
+  unfold left_son_check_list.
+  intros.
+  apply or_not_and.
+  apply not_and_or in H1.
+  destruct H1.
+  + left.
+    revert H1.
+    unfold legal_list_state.
+    simpl fst; simpl snd.
+    rewrite !Zlength_firstn.
+    lia.
+  + assert (2*pos > len2 - 1 \/ 2*pos <= len2 - 1) by lia.
+    destruct H2.
+    - left.
+      unfold legal_list_state.
+      simpl fst; simpl snd.
+      rewrite !Zlength_firstn.
+      apply or_not_and.
+      lia.
+    - right.
+      revert H1.
+      unfold get_list_val.
+      simpl fst; simpl snd.
+      intros.
+      pose proof (Zfirstn_firstn l len2 len1 H).
+      rewrite <- H3.
+      assert (pos < len2) by lia.
+      assert (2 * pos < len2) by lia.
+      pose proof (Znth_firstn (firstn (Z.to_nat len1) l) pos len2 H4).
+      pose proof (Znth_firstn (firstn (Z.to_nat len1) l) (2*pos) len2 H5).
+      rewrite H6, H7.
+      tauto.
+Qed.
+
+Lemma right_son_check_hold: forall l pos len1 len2,
+  len2 <= len1 -> len2 >= 1 ->
+  ~right_son_check_list (firstn (Z.to_nat len1) l, pos) ->
+  ~right_son_check_list (firstn (Z.to_nat len2) l, pos).
+Proof.
+  unfold left_son_check_list.
+  intros.
+  apply or_not_and.
+  apply not_and_or in H1.
+  destruct H1.
+  + left.
+    revert H1.
+    unfold legal_list_state.
+    simpl fst; simpl snd.
+    rewrite !Zlength_firstn.
+    lia.
+  + assert (2*pos+1 > len2 - 1 \/ 2*pos+1 <= len2 - 1) by lia.
+    destruct H2.
+    - left.
+      unfold legal_list_state.
+      simpl fst; simpl snd.
+      rewrite !Zlength_firstn.
+      lia.
+    - right.
+      revert H1.
+      unfold get_list_val.
+      simpl fst; simpl snd.
+      intros.
+      pose proof (Zfirstn_firstn l len2 len1 H).
+      rewrite <- H3.
+      assert (pos < len2) by lia.
+      assert (2*pos+1 < len2) by lia.
+      pose proof (Znth_firstn (firstn (Z.to_nat len1) l) pos len2 H4).
+      pose proof (Znth_firstn (firstn (Z.to_nat len1) l) (2*pos+1) len2 H5).
+      rewrite H6, H7.
+      tauto.
+Qed.
+
+Lemma son_check_hold: forall l pos len1 len2,
+  len2 <= len1 -> len2 >= 1 ->
+  ~left_son_check_list (firstn (Z.to_nat len1) l, pos) /\
+  ~right_son_check_list (firstn (Z.to_nat len1) l, pos) ->
+  ~left_son_check_list (firstn (Z.to_nat len2) l, pos) /\ ~right_son_check_list (firstn (Z.to_nat len2) l, pos).
+Proof.
+  intros.
+  destruct H1.
+  split.
+  + apply (left_son_check_hold l pos len1 len2 H H0 H1).
+  + apply (right_son_check_hold l pos len1 len2 H H0 H2).
+Qed.
+
+(* Lemma MaxHeap_p_coincidence_for_idx: forall l (x1 y1 x2 y2: Z),
+  MaxHeap_p l x1 y1 -> 0 <= x1 <= x2 -> 0 <= y2 <= y1 -> MaxHeap_p l x2 y2.
+Proof.
+  intros.
+  unfold MaxHeap_p in H.
+  unfold MaxHeap_p.
+  intros.
+  apply (son_check_hold l i (y1 + 1) (y2 + 1)); [lia | lia | ].
+  apply H.
+  lia.
+Qed. *)
+
+(* Search sublist.
+Print sublist. *)
+
+Lemma upd_Znth_twice_Zlength: forall {A} (l: list A) p1 p2 v1 v2,
+  0 <= p1 < Zlength l -> 0 <= p2 < Zlength l ->
+  Zlength (upd_Znth p1 (upd_Znth p2 l v2) v1) = Zlength l.
+Proof.
+  intros.
+  rewrite upd_Znth_Zlength.
+  + rewrite upd_Znth_Zlength; lia.
+  + rewrite upd_Znth_Zlength; lia. 
+Qed.
+
+Definition list_swap (l: list Z) (i j: Z) : list Z :=
+  upd_Znth i (upd_Znth j l (Znth i l)) (Znth j l).
+
+Lemma list_swap_Zlength: forall l i j,
+  0 <= i < Zlength l -> 0 <= j < Zlength l ->
+  Zlength (list_swap l i j) = Zlength l.
+Proof.
+  intros.
+  unfold list_swap.
+  apply upd_Znth_twice_Zlength; lia.
+Qed.
+
+Lemma all_int_swap: forall l i j,
+  all_int l ->
+  0 <= i < Zlength l -> 0 <= j < Zlength l ->
+  all_int (list_swap l i j).
+Proof.
+  intros.
+  unfold list_swap.
+  apply all_int_upd_Znth.
+  + apply all_int_upd_Znth; [exact H |  |].
+    - pose proof all_int_Znth _ _ H H0.
+      lia.
+    - pose proof all_int_Znth _ _ H H0.
+      lia.
+  + pose proof all_int_Znth _ _ H H1.
+    lia.
+  + pose proof all_int_Znth _ _ H H1.
+    lia.
+Qed.
+
+Lemma list_swap_rela_correct: forall l i j,
+  0 <= i < Zlength l -> 0 <= j < Zlength l ->
+  list_relation.list_swap i j l (list_swap l i j).
+Proof.
+  intros.
+  unfold list_relation.list_swap.
+  unfold list_swap.
+  split.
+  + rewrite !upd_Znth_Zlength.
+    - reflexivity.
+    - lia.
+    - rewrite upd_Znth_Zlength by lia.
+      lia.
+  + split.
+    assert (i = j \/ i <> j) by lia.
+    destruct H1.
+    - subst.
+      rewrite upd_Znth_same; [reflexivity | ].
+      rewrite upd_Znth_Zlength by lia.
+      lia. 
+    - rewrite upd_Znth_diff.
+      * rewrite upd_Znth_same; [reflexivity | lia].
+      * rewrite upd_Znth_Zlength; lia.
+      * rewrite upd_Znth_Zlength; lia.
+      * lia.
+    - split.
+      assert (i = j \/ i <> j) by lia.
+      destruct H1.
+      * subst.
+        rewrite upd_Znth_same; [reflexivity |].
+        rewrite upd_Znth_Zlength by lia.
+        lia. 
+      * rewrite upd_Znth_same; [reflexivity |].
+        rewrite upd_Znth_Zlength; lia.
+      * intros.
+        destruct H1 as [? [? ?] ].
+        rewrite upd_Znth_diff.
+        rewrite upd_Znth_diff by lia.
+        reflexivity.
+        rewrite upd_Znth_Zlength; lia.
+        rewrite upd_Znth_Zlength; lia.
+        lia.
+Qed.
+
+Lemma firstn_eq_sublist: forall {A: Type} (l: list A) i,
+  firstn (Z.to_nat i) l = sublist 0 i l.
+Proof.
+  intros.
+  unfold sublist.
+  simpl.
+  replace (i - 0) with i by lia.
+  tauto.
+Qed.
+
+Lemma list_swap_firstn: forall l i j len,
+  0 <= i < len -> 0 <= j < len -> len <= Zlength l ->
+  firstn (Z.to_nat len) (list_swap l i j) = list_swap (firstn (Z.to_nat len) l) i j.
+Proof.
+  intros.
+  unfold list_swap.
+  rewrite !firstn_eq_sublist.
+  rewrite !sublist_upd_Znth_lr; try lia.
+  + rewrite !Znth_sublist; try lia.
+    replace (i - 0) with i by lia.
+    replace (j - 0) with j by lia.
+    replace (i + 0) with i by lia.
+    replace (j + 0) with j by lia.
+    reflexivity.
+  + rewrite upd_Znth_Zlength; lia.  
+Qed.
+
+Lemma list_swap_rela_correct_firstn: forall l i j len,
+  0 <= i < len -> 0 <= j < len -> len <= Zlength l ->
+  list_relation.list_swap i j (firstn (Z.to_nat len) l) (firstn (Z.to_nat len) (list_swap l i j)).
+Proof.
+  intros.
+  rewrite list_swap_firstn by lia.
+  apply list_swap_rela_correct.
+  + rewrite Zlength_firstn.
+    lia.
+  + rewrite Zlength_firstn.
+    lia.  
+Qed.
+
+Lemma list_swap_eq: forall l i j,
+  0 <= i < Zlength l -> 0 <= j < Zlength l ->
+  list_swap l i j = list_swap l j i.
+Proof.
+  intros.
+  eapply Znth_eq_ext.
+  + rewrite !list_swap_Zlength by lia.
+    reflexivity.
+  + intros.
+    unfold list_swap.
+    assert (i = i0 \/ i <> i0) by lia.
+    destruct H2.
+    - subst.
+      rewrite upd_Znth_same.
+      assert (j = i0 \/ j <> i0) by lia.
+      destruct H2.
+      * subst.
+        rewrite upd_Znth_same; [reflexivity | rewrite upd_Znth_Zlength; lia].
+      * rewrite upd_Znth_diff.
+        rewrite upd_Znth_same; [reflexivity | lia ].
+        rewrite upd_Znth_Zlength; lia.
+        rewrite upd_Znth_Zlength; lia.
+        lia.
+      * rewrite upd_Znth_Zlength; lia.
+    - rewrite list_swap_Zlength in H1 by lia.
+      rewrite upd_Znth_diff.
+      assert (j = i0 \/ j <> i0) by lia. 
+      destruct H3.
+      * subst.
+        rewrite !upd_Znth_same; [reflexivity | rewrite upd_Znth_Zlength; lia | lia].
+      * rewrite !upd_Znth_diff; try lia.
+        ++ rewrite upd_Znth_Zlength by lia; lia.
+        ++ rewrite upd_Znth_Zlength by lia; lia.
+      * rewrite upd_Znth_Zlength; lia.
+      * rewrite upd_Znth_Zlength; lia.
+      * lia.     
+Qed.
+
+Lemma Zlor_add_one: forall x,
+  x >= 0 -> Z.lor (2 * x) 1 = 2 * x + 1.
+Proof.
+  intros.
+  induction x; simpl.
+  + reflexivity.
+  + reflexivity.
+  + lia.   
+Qed.
+
+(* Lemma up_pos_in_range: forall l l' x y size,
+  (up l size x y l') -> (1 <= y /\ y <= size).
+Proof.
+  intros.
+  unfold up,heap_list_up in H.
+  induction H.
+  induction x0.
+  + unfold nsteps in H.
+Qed. *)
+
+
+(* Lemma MaxHeap_p_coincidence_for_list: forall l l' x y,
+  MaxHeap_p l x y ->
+  (forall i, x <= i <= y -> Znth i l = Znth i l') ->
+  MaxHeap_p l' x y.
+Proof. Admitted.
+
+Lemma MaxHeap_up_succeed: forall l l' pos size,
+  Zlength l >= size + 1 -> size >= 1 ->
+  MaxHeap l (pos-1) -> MaxHeap_p l pos size -> list_up_succeed ((firstn (Z.to_nat (size+1)) l),pos) (l',(pos/2))
+  -> MaxHeap l' (pos/2 - 1) /\ MaxHeap_p l' (pos/2) size.
+Proof.
+  intros.
+  unfold list_up_succeed in H3.
+  unfold legal_list_state in H3.
+  simpl fst in H3.
+  simpl snd in H3.
+  rewrite !Zlength_firstn in H3.
+  replace (Z.min (Z.max 0 (size + 1)) (Zlength l)) with (size + 1) in H3 by lia.
+  destruct H3 as [? [?  [? [? [? ?] ] ] ] ].
+  split.
+  + Admitted.
+
+Lemma MaxHeap_up_fail: forall l pos size, 
+  MaxHeap l (pos-1) -> MaxHeap_p l pos size
+  -> list_up_fail ((firstn (Z.to_nat (size + 1)) l), pos) ((firstn (Z.to_nat (size + 1)) l), pos)
+  -> MaxHeap l size.
+Proof.
+  intros.
+  unfold list_up_fail in H1.
+  revert H1; unfold_RELS_tac; intros.
+  destruct H1; clear H2.
+  destruct H1, H2.
+  + unfold snd in H2; subst.
+    apply H0.
+  + revert H2; unfold fst, snd; intros.
+    destruct H2.
+    Admitted. *)
+
+Lemma offset_val_field_address:
+  forall T pos len a,
+    0 <= pos < len ->
+    field_compatible (tarray T len) [] a ->
+    offset_val (sizeof T * pos) a = field_address (tarray T len) [ArraySubsc pos] a.
+Proof.
+  intros.
+  assert (field_compatible (tarray T len) [ArraySubsc pos] a). {
+    apply field_compatible_cons.
+    split; [lia | tauto].
+  }
+  pose proof field_compatible_field_address _ _ _ H1.
+  rewrite H2.
+  tauto. 
+Qed.
+
+Lemma field_address_array_smaller:
+  forall T size small_size a pos,
+    0 <= small_size <= size -> 0 <= pos < small_size ->
+    field_compatible (tarray T size) [] a ->
+    field_address (tarray T size) [ArraySubsc pos] a =
+    field_address (tarray T small_size) [ArraySubsc pos] a.
+Proof.
+  intros.
+  rewrite <- offset_val_field_address; [ | lia | tauto].
+  eapply field_compatible_Tarray_split in H1.
+  + destruct H1.
+    rewrite <- offset_val_field_address; [tauto | lia | apply H1].
+  + lia.
+Qed.
+
+Lemma field_address_array_relocate:
+  forall T size a p1 p2,
+    0 <= p1 < size -> 0 <= p2 < size -> p1 <= p2 ->
+    field_compatible (tarray T size) [] a ->
+    field_address (tarray T size) [ArraySubsc p2] a =
+    field_address (tarray T (size - p1)) [ArraySubsc (p2 - p1)] (field_address0 (tarray T size) [ArraySubsc p1] a).
+Proof.
+  intros.
+  rewrite field_address0_offset.
+  2: {
+    apply field_compatible0_cons.
+    simpl; split; [lia | tauto].
+  }
+  rewrite !field_address_offset.
+  3: {
+    apply field_compatible_cons.
+    simpl; split; [lia | tauto].
+  }
+  2: {
+    simpl.
+    apply field_compatible_cons.
+    simpl; split; [lia |].
+    pose proof field_compatible_Tarray_split T p1 size a ltac:(lia).
+    apply H3 in H2; destruct H2.
+    rewrite field_address0_offset in H4.
+    + tauto.
+    + apply field_compatible0_cons.
+      simpl; split; [lia | tauto].  
+  }
+  simpl.
+  rewrite offset_offset_val.
+  f_equal; lia.
+Qed.
+
+Lemma int_array_with_two_holes: forall a l size p1 p2,
+  0 <= p1 < size -> p1 < p2 < size -> size >= 0 ->
+  store_int_array a l size
+  |-- (store_int (field_address (tarray tint size) [ArraySubsc p1] a) (Znth p1 l) *
+       store_int (field_address (tarray tint size) [ArraySubsc p2] a) (Znth p2 l) *
+       SingletonHole.array_with_hole Tsh tint 0 (size - p2) (map Vint (map IntRepr (sublist p2 size l)))
+         (field_address0 (tarray tint size) [ArraySubsc p2] a) *
+       SingletonHole.array_with_hole Tsh tint p1 p2 (map Vint (map IntRepr (sublist 0 p2 l))) a)%logic.
+Proof.
+  intros.
+  sep_apply list_length; [lia | ].
+  Intros.
+  entailer!.
+  pose proof split2_data_at_Tarray Tsh tint (Zlength l) p2.
+  erewrite H5; [| lia | rewrite H4; lia | | |].
+  2: rewrite sublist_same; [tauto | tauto | rewrite H4; tauto].
+  2: rewrite !sublist_map; reflexivity.
+  2: rewrite !sublist_map; reflexivity.
+  change (Tarray tint p2 noattr) with (tarray tint p2).
+  change (Tarray tint (Zlength l - p2) noattr) with (tarray tint (Zlength l - p2)).
+  pose proof SingletonHole.array_with_hole_intro Tsh tint p1 p2 (map Vint (map Int.repr (sublist 0 p2 l))) a ltac:(lia).
+  rewrite !Znth_map in H6.
+  2: rewrite Zlength_sublist by lia; lia.
+  2: rewrite Zlength_map, Zlength_sublist by lia; lia.
+  rewrite !Znth_sublist in H6 by lia.
+  replace (p1 + 0) with p1 in H6 by lia.
+  rewrite (field_address_array_smaller _ _ p2 _ _); [| lia | lia | tauto].
+  sep_apply H6; entailer!.
+  change (Tarray tint (Zlength l) noattr) with (tarray tint (Zlength l)).
+  pose proof SingletonHole.array_with_hole_intro Tsh tint 0 (Zlength l - p2).
+  sep_apply H12; [lia |].
+  rewrite !Znth_map.
+  2: rewrite Zlength_sublist by lia; lia.
+  2: rewrite Zlength_map, Zlength_sublist by lia; lia.
+  rewrite !Znth_sublist by lia.
+  replace (0 + p2) with p2 by lia.
+  replace 0 with (p2 - p2) at 1 by lia.
+  rewrite <- (field_address_array_relocate _ _ _ p2 p2); [| lia | lia | lia | tauto].
+  entailer!.
+Qed.
+
+Lemma int_array_with_two_holes_inv: forall a l p1 p2 v1 v2,
+  0 <= p1 < Zlength l -> p1 < p2 < Zlength l ->
+  field_compatible (tarray tint (Zlength l)) [] a ->
+  (store_int (field_address (tarray tint (Zlength l)) [ArraySubsc p1] a) v1 *
+   store_int (field_address (tarray tint (Zlength l)) [ArraySubsc p2] a) v2 *
+   SingletonHole.array_with_hole Tsh tint 0 (Zlength l - p2) (map Vint (map IntRepr (sublist p2 (Zlength l) l)))
+     (field_address0 (tarray tint (Zlength l)) [ArraySubsc p2] a) *
+   SingletonHole.array_with_hole Tsh tint p1 p2 (map Vint (map IntRepr (sublist 0 p2 l))) a)%logic
+  |-- store_int_array a (upd_Znth p1 (upd_Znth p2 l v2) v1) (Zlength l).
+Proof.
+  intros.
+  pose proof split2_data_at_Tarray Tsh tint (Zlength l) p2.
+  erewrite H2; [ | lia | | | |].
+  3: {
+    rewrite sublist_same; [reflexivity | lia | rewrite !Zlength_map].
+    rewrite !upd_Znth_twice_Zlength by lia.
+    reflexivity.
+  }
+  2: {
+    rewrite !Zlength_map.
+    rewrite upd_Znth_twice_Zlength by lia.
+    lia.
+  }
+  2: rewrite !sublist_map; reflexivity.
+  2: rewrite !sublist_map; reflexivity.
+  change (Tarray tint p2 noattr) with (tarray tint p2).
+  change (Tarray tint (Zlength l - p2) noattr) with (tarray tint (Zlength l - p2)).
+  pose proof SingletonHole.array_with_hole_elim Tsh tint p1 p2
+    (Vint(IntRepr(v1))) (map Vint (map IntRepr (sublist 0 p2 l))) a.
+  rewrite !upd_Znth_map in H3.
+  replace (sublist 0 p2 (upd_Znth p1 (upd_Znth p2 l v2) v1))
+    with (upd_Znth p1 (sublist 0 p2 l) v1).
+  rewrite (field_address_array_smaller _ _ p2 _ _); [| lia | lia | tauto].
+  2: {
+    rewrite sublist_upd_Znth_lr; [ | lia | rewrite upd_Znth_Zlength; lia].
+    rewrite sublist_upd_Znth_l by lia.
+    replace (p1 - 0) with p1 by lia.
+    tauto.
+  }
+  sep_apply H3; entailer!.
+  pose proof SingletonHole.array_with_hole_elim Tsh tint 0 (Zlength l - p2)
+    (Vint(IntRepr(v2))) (map Vint (map IntRepr (sublist p2 (Zlength l) l)))
+    (field_address0 (Tarray tint (Zlength l) noattr) [ArraySubsc p2] a).
+  rewrite !upd_Znth_map in H9.
+  replace (sublist p2 (Zlength l) (upd_Znth p1 (upd_Znth p2 l v2) v1))
+    with (upd_Znth 0 (sublist p2 (Zlength l) l) v2).
+  rewrite (field_address_array_relocate _ _ _ p2 p2); [| lia | lia | lia | tauto].
+  2: {
+    rewrite sublist_upd_Znth_r; [ | lia | rewrite upd_Znth_Zlength; lia].
+    rewrite sublist_upd_Znth_lr by lia.
+    replace (p2 - p2) with 0 by lia.
+    tauto.
+  }
+  replace (p2 - p2) with 0 by lia.
+  sep_apply H9.
+  entailer!.
+Qed.
