heap/down/path11_verif.v
@@ -1,0 +1,68 @@
+Require Import utils.VSTALib.
+
+Require Import heap.program.
+Require Import heap.definitions.
+Require Import heap.annotation.
+Require Import SetsClass.SetsClass.
+Require Import Classical_Prop.
+Require heap.down.path11.
+
+Module SH_Proof <: STRAIGHTLINE_HOARE_TRIPLE_PROOF.
+
+Include heap.down.path11.
+
+Theorem proof: functional_correctness_statement.
+Proof.
+  cbv delta [functional_correctness_statement].
+  intros.
+  Intros Hl0 pos1 a pos size.
+  subst.
+  sep_apply list_length; [lia | ].
+  Intros.
+  sep_apply int_array_is_ptr; [lia | ].
+  Intros.
+  forward.
+  forward.
+  assert ((Int.shl (IntRepr pos1) (IntRepr 1)) = Int.repr (2 * pos1)). {
+    unfold Int.shl.
+    unfold Z.shiftl.
+    simpl.
+    rewrite Int.unsigned_repr by rep_lia.
+    f_equal; lia.
+  }
+  rewrite H3, Int.signed_repr in H1 by rep_lia.
+  assert (Int.unsigned (Int.shl (IntRepr pos1) (IntRepr 1)) = 2 * pos1). {
+    rewrite H3.
+    rewrite Int.unsigned_repr by rep_lia.
+    reflexivity.
+  }
+  forward.
+  rewrite H12.
+  forward.
+  forward.
+  forward.
+  rewrite H3 in H14.
+  assert (Int.or (IntRepr (2 * pos1)) (IntRepr 1) = IntRepr(2 * pos1 + 1)). {
+    unfold Int.or.
+    f_equal.
+    rewrite !Int.unsigned_repr by rep_lia.
+    apply Zlor_add_one; lia.
+  }
+  rewrite H15 in H14.
+  rewrite Int.signed_repr in H14 by rep_lia.
+  assert (Int.unsigned (Int.or (Int.shl (IntRepr pos1) (IntRepr 1)) (IntRepr 1))  = 2 * pos1 + 1). {
+    rewrite H3, H15.
+    rewrite Int.unsigned_repr by rep_lia.
+    reflexivity.
+  }
+  forward.
+  rewrite H16.
+  forward.
+  forward.
+  forward.
+  rewrite H3, H15.
+  forward.
+  lia.
+Qed.
+
+End SH_Proof.
