heap/down/path2_verif.v
@@ -1,0 +1,130 @@
+Require Import utils.VSTALib.
+
+Require Import heap.program.
+Require Import heap.definitions.
+Require Import heap.annotation.
+Require Import SetsClass.SetsClass.
+Require Import Classical_Prop.
+Require heap.down.path2.
+
+Module SH_Proof <: STRAIGHTLINE_HOARE_TRIPLE_PROOF.
+
+Include heap.down.path2.
+
+Theorem proof: functional_correctness_statement.
+Proof.
+  cbv delta [functional_correctness_statement].
+  intros.
+  Intros Hl0 pos1 a pos size.
+  subst.
+  sep_apply list_length; [lia | ].
+  Intros.
+  sep_apply int_array_is_ptr; [lia | ].
+  Intros.
+  forward.
+  forward.
+  assert ((Int.shl (IntRepr pos1) (IntRepr 1)) = Int.repr (2 * pos1)). {
+    unfold Int.shl.
+    unfold Z.shiftl.
+    simpl.
+    rewrite Int.unsigned_repr by rep_lia.
+    f_equal; lia.
+  }
+  rewrite H3, Int.signed_repr in H1 by rep_lia.
+  assert (Int.unsigned (Int.shl (IntRepr pos1) (IntRepr 1)) = 2 * pos1). {
+    rewrite H3.
+    rewrite Int.unsigned_repr by rep_lia.
+    reflexivity.
+  }
+  forward.
+  rewrite H12.
+  forward.
+  forward.
+  forward.
+  rewrite H3.
+  forward.
+  rewrite H3 in H14.
+  assert (Int.or (IntRepr (2 * pos1)) (IntRepr 1) = IntRepr(2 * pos1 + 1)). {
+    unfold Int.or.
+    f_equal.
+    rewrite !Int.unsigned_repr by rep_lia.
+    apply Zlor_add_one; lia.
+  }
+  rewrite H15 in H14.
+  rewrite Int.signed_repr in H14 by rep_lia.
+  assert (Int.unsigned (Int.or (Int.shl (IntRepr pos1) (IntRepr 1)) (IntRepr 1))  = 2 * pos1 + 1). {
+    rewrite H3, H15.
+    rewrite Int.unsigned_repr by rep_lia.
+    reflexivity.
+  }
+  forward.
+  rewrite H16.
+  forward.
+  forward.
+  forward.
+  assert_PROP (field_compatible (tarray tint Maxsize) [] a0) by entailer!.
+  forward_call (Znth (2 * pos1) Hl0, Znth pos1 Hl0, 
+                field_address (tarray tint Maxsize) [ArraySubsc (2 * pos1)] a0,
+                field_address (tarray tint Maxsize) [ArraySubsc pos1] a0,
+                field_address (tarray tint Maxsize) [ArraySubsc pos1] a0,
+                field_address (tarray tint Maxsize) [ArraySubsc (2 * pos1)] a0).
+  {
+    entailer!.
+    split.
+    + f_equal; apply offset_val_field_address; [lia | tauto].
+    + f_equal; apply offset_val_field_address; [lia | tauto].
+  }
+  {
+    sep_apply (int_array_with_two_holes a0 Hl0 Maxsize pos1 (2 * pos1));
+      [lia | lia | lia | entailer!].  
+  }
+  forward.
+  Exists (list_swap Hl0 pos1 (2 * pos1)) (2 * pos1) a0 (Vint (IntRepr (2 * pos1))) (Vint (IntRepr size0)).
+  entailer!.
+  2: {
+    sep_apply (int_array_with_two_holes_inv a0 Hl0 pos1 (2 * pos1) (Znth (2 * pos1) Hl0) (Znth pos1 Hl0));
+      [lia | lia | entailer!].
+  }
+  split.
+  2: apply all_int_swap; [tauto | lia | lia].
+  unfold down_inv.
+  etransitivity_n1; [apply H | ].
+  rewrite !Int.signed_repr in H13, H17.
+  2: apply all_int_Znth; [tauto | lia].
+  2: apply all_int_Znth; [tauto | lia].
+  2: apply all_int_Znth; [tauto | lia].
+  2: apply all_int_Znth; [tauto | lia].
+  unfold list_relation.list_down_succeed.
+  assert (Znth (2 * pos1 + 1) Hl0 <= Znth pos1 Hl0 \/ Znth (2 * pos1 + 1) Hl0 > Znth pos1 Hl0) by lia.
+  destruct H0.
+  {
+    left.
+    list_relation.try_list_unfold_witout_Z.
+    split; split; try split.
+    + rewrite Zlength_firstn; lia.
+    + lia.
+    + rewrite !Znth_firstn by lia; lia.
+    + apply or_not_and; right.
+      rewrite !Znth_firstn by lia.
+      lia.
+    + apply list_swap_rela_correct_firstn; lia.
+    + lia.  
+  }
+  {
+    right; left.
+    list_relation.try_list_unfold_witout_Z.
+    repeat split.
+    + rewrite Zlength_firstn; lia.
+    + lia.
+    + rewrite !Znth_firstn by lia; lia.
+    + rewrite Zlength_firstn; lia.
+    + lia.
+    + rewrite !Znth_firstn by lia; lia.
+    + left; split.
+      - rewrite !Znth_firstn by lia; lia.
+      - split; [ | tauto].
+        apply list_swap_rela_correct_firstn; lia.
+  }
+Qed.
+
+End SH_Proof.
