heap/pop/ret_path1_verif.v
@@ -1,0 +1,68 @@
+Require Import utils.VSTALib.
+
+Require Import heap.program.
+Require Import heap.definitions.
+Require Import heap.annotation.
+Require heap.pop.ret_path1.
+
+Module SH_Proof <: STRAIGHTLINE_HOARE_TRIPLE_PROOF.
+
+Include heap.pop.ret_path1.
+
+Theorem proof: functional_correctness_statement.
+Proof.
+  cbv delta [functional_correctness_statement].
+  intros; Intros; subst.
+  forward. forward. forward.
+  sep_apply list_length; [lia|].
+  Intros.
+  forward. forward. forward. forward. forward. forward. forward.
+  forward_call ((size0-1), 1, a0, Maxsize, upd_Znth 1 Hl (Znth size0 Hl), a0, (Vint (IntRepr 1)), (Vint (IntRepr (size0-1)))).
+  + rewrite ! upd_Znth_map.
+    entailer!.
+  + split; [reflexivity|]. 
+    split; [reflexivity|].
+    split; [reflexivity|].
+    split; [lia|].
+    split; [lia|].
+    split; [lia|].
+    split; [lia|].
+    split; [lia|].
+    split; [lia|].
+    pose proof all_int_Znth Hl size0 H5 ltac:(lia).
+    destruct H7.
+    apply all_int_upd_Znth; tauto.
+  + Intros vret; destruct vret as [l2 pos1]; subst.
+    forward.
+    Exists l2 (size0-1) (Vint (IntRepr (0))).
+    entailer!.
+    split.
+    - unfold pop.
+      right.
+      split; [lia|].
+      unfold heap_pop; right.
+      split; [rewrite Zlength_firstn; lia|].
+      exists pos1.
+      unfold down in H7.
+      unfold fst, snd in H7.
+      rewrite Zlength_firstn.
+      replace (Z.max 0 (size0 + 1)) with (size0 + 1) by lia.
+      replace (Z.min (size0 + 1) (Zlength Hl)) with (size0 + 1) by lia.
+      replace (size0 + 1 - 1) with size0 by lia.
+      replace (size0 - 1 + 1) with size0 in H7 by lia.
+      assert (firstn (Z.to_nat size0) (upd_Znth 1 Hl (Znth size0 Hl)) = firstn (Z.to_nat size0)
+        (upd_Znth 1 (firstn (Z.to_nat (size0 + 1)) Hl)
+          (Znth size0 (firstn (Z.to_nat (size0 + 1)) Hl)))); [|rewrite <- H15; tauto].
+      rewrite ! Znth_firstn; [|lia].
+      rewrite ! firstn_eq_sublist.
+      rewrite ! sublist_upd_Znth_lr; try lia; [|rewrite Zlength_sublist; lia].
+      rewrite ! sublist_firstn.
+      rewrite List.firstn_firstn.
+      replace (Init.Nat.min (Z.to_nat size0) (Z.to_nat (size0 + 1))) with (Z.to_nat size0) by lia.
+      reflexivity.
+    - split.
+      * destruct size0; [lia | unfold pop_length; reflexivity| lia ].
+      * destruct size0; [lia | unfold pop_result; reflexivity| lia ].
+Qed.
+
+End SH_Proof.
