heap/pop/ret_path2.v
@@ -1,0 +1,63 @@
+From Coq Require Import String List ZArith.
+From compcert Require Import Coqlib Integers Floats AST Ctypes Cop Clight Clightdefs.
+Require Import Csplit.semantics.
+Require Import utils.AClightNotations.
+Require VST.floyd.proofauto.
+Require Import FloydSeq.proofauto.
+Require Import Csplit.strong.
+Require Import FloydSeq.client_lemmas.
+Require Import Csplit.strongSoundness.
+Require Import Csplit.AClightFunc.
+Local Open Scope Z_scope.
+Import AClightNotations.
+Require Import heap.program.
+Require Import heap.definitions.
+Require Import heap.annotation.
+Import compcert.cfrontend.Clight.
+
+Definition functional_correctness_statement: Prop :=
+  forall (Espec: OracleKind) Hl Maxsize size0 size_p a0 a' size',
+  let Delta_specs := Delta_specs_pop in
+  let Delta := Delta_pop Delta_specs in
+  semax Delta (PROP ((size' = size_p); (a' = a0); (Z.le (Z.add size0 1) Maxsize); (Z.le 0 size0); (Z.le (Z.mul 2 Maxsize) (Int.max_signed )); (Z.le 1 Maxsize); (all_int Hl))
+  LOCAL (temp _a a'; temp _size size')
+  SEP ((store_int_array a0 Hl Maxsize); (store_int size_p size0)))
+  (Ssequence
+    (Sset _t'6 (Ederef (Etempvar _size (tptr tint)) tint))
+    (Ssequence
+      (Sifthenelse (Ebinop Oeq (Etempvar _t'6 tint)
+                     (Econst_int (Int.repr 0) tint) tint)
+        Sbreak
+        Sskip)
+      (Ssequence
+        (Sset _t'4 (Ederef (Etempvar _size (tptr tint)) tint))
+        (Ssequence
+          (Sset _t'5
+            (Ederef
+              (Ebinop Oadd (Etempvar _a (tptr tint)) (Etempvar _t'4 tint)
+                (tptr tint)) tint))
+          (Ssequence
+            (Sassign
+              (Ederef
+                (Ebinop Oadd (Etempvar _a (tptr tint))
+                  (Econst_int (Int.repr 1) tint) (tptr tint)) tint)
+              (Etempvar _t'5 tint))
+            (Ssequence
+              (Sset _t'3 (Ederef (Etempvar _size (tptr tint)) tint))
+              (Ssequence
+                (Sassign (Ederef (Etempvar _size (tptr tint)) tint)
+                  (Ebinop Osub (Etempvar _t'3 tint)
+                    (Econst_int (Int.repr 1) tint) tint))
+                (Ssequence
+                  (Sset _t'1 (Ederef (Etempvar _size (tptr tint)) tint))
+                  (Ssequence
+                    (Sifthenelse (Ebinop Oge (Etempvar _t'1 tint)
+                                   (Econst_int (Int.repr 1) tint) tint)
+                      Sbreak
+                      Sskip)
+                    (Sreturn (Some (Econst_int (Int.repr 0) tint))))))))))))
+  (return_split_assert (RA_return (frame_ret_assert (function_body_ret_assert tint 
+  (EX Hl_final size1 __return,
+    (PROP ((pop Hl size0 Hl_final); (size1 = (pop_length Hl size0)); (__return = (Vint (IntRepr (pop_result Hl size0)))))
+    LOCAL (temp ___return __return)
+    SEP ((store_int_array a0 Hl_final Maxsize); (store_int size_p size1))))%assert) (stackframe_of f_pop)))).
