heap/pop/ret_path2_verif.v
@@ -1,0 +1,40 @@
+Require Import utils.VSTALib.
+
+Require Import heap.program.
+Require Import heap.definitions.
+Require Import heap.annotation.
+Require heap.pop.ret_path2.
+
+Module SH_Proof <: STRAIGHTLINE_HOARE_TRIPLE_PROOF.
+
+Include heap.pop.ret_path2.
+
+Theorem proof: functional_correctness_statement.
+Proof.
+  cbv delta [functional_correctness_statement].
+  intros; Intros; subst.
+  sep_apply list_length; [lia|]; Intros.
+  forward. forward. forward. forward. forward. forward. forward. forward. forward. forward.
+  Exists (upd_Znth 1 Hl (Znth size0 Hl)) (size0-1) (Vint (IntRepr (0))).
+  rewrite ! upd_Znth_map.
+  entailer!.
+  split.
+  + unfold pop.
+    right.
+    split; [lia|].
+    assert (size0 = 1) by lia.
+    subst.
+    unfold heap_pop.
+    left.
+    split.
+    - rewrite Zlength_firstn.
+      lia. 
+    - rewrite Zlength_firstn.
+      rewrite upd_Znth_Zlength; [|lia].
+      lia.
+  + split.
+    - destruct size0; [lia | unfold pop_length; reflexivity| lia ].
+    - destruct size0; [lia | unfold pop_result; reflexivity| lia ].
+Qed.
+
+End SH_Proof.
