heap/up/path1_verif.v
@@ -1,0 +1,109 @@
+Require Import utils.VSTALib.
+
+Require Import heap.program.
+Require Import heap.definitions.
+Require Import heap.annotation.
+Require heap.up.path1.
+Require Import SetsClass.SetsClass.
+
+Module SH_Proof <: STRAIGHTLINE_HOARE_TRIPLE_PROOF.
+
+Include heap.up.path1.
+
+Theorem proof: functional_correctness_statement.
+Proof.
+  cbv delta [functional_correctness_statement].
+  intros.
+  Intros Hl0 pos1 a pos.
+  subst.
+  sep_apply list_length; [lia | ]; Intros.
+  forward.
+  forward.
+  assert (1 <= pos1 / 2 /\ pos1 / 2 < pos1). {
+    split.
+    + pose proof Z.div_le_lower_bound pos1 2 1 ltac:(lia) ltac:(lia).
+      lia.
+    + pose proof Z.div_lt_upper_bound pos1 2 pos1 ltac:(lia) ltac:(lia).
+      lia.
+  }
+  assert ((Int.shr (IntRepr pos1) (IntRepr 1)) = Int.repr (pos1 / 2)). {
+    unfold Int.shr.
+    rewrite Int.signed_repr by rep_lia.
+    rewrite Int.unsigned_repr by rep_lia.
+    unfold Z.shiftr.
+    simpl.
+    rewrite Z.div2_div.
+    reflexivity.
+  }
+  assert (Int.unsigned (Int.shr (IntRepr pos1) (IntRepr 1)) = pos1 / 2). {
+    rewrite H12.
+    rewrite Int.unsigned_repr by rep_lia.
+    reflexivity.
+  }
+  forward.
+  rewrite H12.
+  forward.
+  sep_apply int_array_is_ptr; [lia | ]; Intros.
+  assert_PROP (field_compatible (tarray tint (Zlength Hl0)) [] a0) by entailer!.
+  forward_call (Znth (pos1 / 2) Hl0, Znth pos1 Hl0, 
+                field_address (tarray tint Maxsize) [ArraySubsc (pos1 / 2)] a0,
+                field_address (tarray tint Maxsize) [ArraySubsc pos1] a0,
+                field_address (tarray tint Maxsize) [ArraySubsc pos1] a0,
+                field_address (tarray tint Maxsize) [ArraySubsc (pos1 / 2)] a0).
+  {
+    entailer!.
+    split.
+    + f_equal.
+      apply offset_val_field_address; [lia | tauto].
+    + f_equal.
+      rewrite H12, floyd.forward.sem_add_pi'.
+      - apply offset_val_field_address; [lia | tauto].
+      - tauto. 
+      - tauto.
+      - rep_lia.
+  }
+  {
+    sep_apply (int_array_with_two_holes a0 Hl0 Maxsize (pos1 / 2) pos1);
+      [lia | lia | lia |].
+    entailer!.
+  }
+  forward.
+  Exists (list_swap Hl0 (pos1 / 2) pos1) (pos1 / 2) a0 (Vint (IntRepr (pos1 / 2))).
+  entailer!.
+  2: {
+    sep_apply (int_array_with_two_holes_inv a0 Hl0 (pos1 / 2) pos1 (Znth pos1 Hl0) (Znth (pos1 / 2) Hl0));
+      [ lia | lia | entailer! ].
+  }
+  split.
+  2: {
+    split; [ | f_equal; rewrite H12; reflexivity].
+    apply all_int_swap; [tauto | lia | lia ].
+  }
+  unfold up_inv.
+  etransitivity_n1; [apply H | ].
+  unfold list_relation.list_up_succeed.
+  unfold list_relation.legal_list_state.
+  unfold list_relation.get_list_val.
+  simpl; split.
+  + split; [| lia].
+    rewrite Zlength_firstn.
+    lia.
+  + split.
+    - split; [| lia].
+      rewrite Zlength_firstn.
+      assert (Zlength (list_swap Hl0 (pos1 / 2) pos1) = Zlength Hl0)
+        by (rewrite list_swap_Zlength; lia).
+      lia.
+    - split; [lia | ].
+      split; [lia | ].
+      split.
+      * rewrite !Int.signed_repr in H14.
+        ++ rewrite !Znth_firstn by lia.
+           lia.
+        ++ apply all_int_Znth; [tauto | lia].
+        ++ apply all_int_Znth; [tauto | lia].
+      * rewrite list_swap_eq by lia.
+        apply list_swap_rela_correct_firstn; lia.
+Qed.
+
+End SH_Proof.
