heap/up/path3_verif.v
@@ -1,0 +1,71 @@
+Require Import utils.VSTALib.
+
+Require Import heap.program.
+Require Import heap.definitions.
+Require Import heap.annotation.
+Require Import SetsClass.SetsClass.
+Require heap.up.path3.
+
+Module SH_Proof <: STRAIGHTLINE_HOARE_TRIPLE_PROOF.
+
+Include heap.up.path3.
+
+Theorem proof: functional_correctness_statement.
+Proof.
+  cbv delta [functional_correctness_statement].
+  intros; Intros Hl0 pos1 a pos; subst.
+  forward.
+  sep_apply list_length; [lia|]; Intros.
+  forward.
+  assert (1 <= pos1 / 2 /\ pos1 / 2 < pos1). {
+    split.
+    + pose proof Z.div_le_lower_bound pos1 2 1 ltac:(lia) ltac:(lia).
+      lia.
+    + pose proof Z.div_lt_upper_bound pos1 2 pos1 ltac:(lia) ltac:(lia).
+      lia.
+  }
+  assert ((Int.shr (IntRepr pos1) (IntRepr 1)) = Int.repr (pos1 / 2)). {
+    unfold Int.shr.
+    rewrite Int.signed_repr by rep_lia.
+    rewrite Int.unsigned_repr by rep_lia.
+    unfold Z.shiftr.
+    simpl.
+    rewrite Z.div2_div.
+    reflexivity.
+  }
+  assert (Int.unsigned (Int.shr (IntRepr pos1) (IntRepr 1)) = pos1 / 2). {
+    rewrite H12.
+    rewrite Int.unsigned_repr by rep_lia.
+    reflexivity.
+  }
+  forward. forward. forward.
+  Exists Hl0 pos1.
+  entailer!.
+  unfold up.
+  unfold list_relation.heap_list_up.
+  unfold up_inv in H. 
+  unfold_RELS_tac.
+  exists (firstn (Z.to_nat (size0 + 1)) Hl0, pos1).
+  split; [apply H|].
+  unfold list_relation.list_up_fail.
+  unfold_RELS_tac.
+  split; [|reflexivity].
+  split.
+  + unfold list_relation.legal_list_state.
+    simpl.
+    split; [|tauto].
+    rewrite Zlength_firstn.
+    replace (Z.max 0 (size0 + 1)) with (size0 + 1) by lia.
+    lia.
+  + right; simpl.
+    split; [lia|].
+    unfold list_relation.get_list_val; simpl.
+    rewrite H13 in H14.
+    rewrite ! Znth_firstn; [ | lia | lia].
+    pose proof all_int_Znth Hl0 pos1 H10 ltac:(lia).
+    pose proof all_int_Znth Hl0 (pos1/2) H10 ltac:(lia).
+    rewrite ! Int.signed_repr in H14 by tauto.
+    lia.
+Qed.
+
+End SH_Proof.
